src/3d/prelude/EverParse3d.InputBuffer.fst
@@ -13,20 +13,19 @@ open LowParse.Low.Base
 
 let input_buffer_t = Aux.input_buffer
 
-let slice_of x = { LPL.base = x.Aux.base; LPL.len = x.Aux.len }
-
-let slice_length x = x.Aux.len
+let slice_of #len x = { LPL.base = x.Aux.base; LPL.len = len }
 
 let perm_of x = x.Aux.perm
 
-let truncate_input_buffer x len =
-  { Aux.base = x.Aux.base; Aux.perm = x.Aux.perm; Aux.len = len }
+let truncate_input_buffer #len0 x len =
+  { Aux.base = x.Aux.base; Aux.perm = x.Aux.perm; }
 
 let drop sl from to =
   R.drop sl.Aux.perm from to
 
-let read_with_perm #k #t #p r j sl pos =
-  [@inline_let] let sl' : LPL.slice triv triv = { LPL.base = sl.Aux.base; LPL.len = sl.Aux.len } in
+(* TODO: remove the slice here *)
+let read_with_perm #k #t #p r j #len sl pos =
+  [@inline_let] let sl' : LPL.slice triv triv = { LPL.base = sl.Aux.base; LPL.len = len } in
   let pos' = j sl' pos in
   drop sl pos pos' ;
   r sl' pos
